Capless/Weakening/TypedCont/Type.lean
@@ -14,6 +14,10 @@ theorem EType.tweaken_weaken (E : EType n m k) :
   E.weaken.tweaken = E.tweaken.weaken := by
   simp [EType.tweaken, EType.weaken, EType.trename_rename_comm]
 
+theorem EType.tweaken_cweaken (E : EType n m k) :
+  E.cweaken.tweaken = E.tweaken.cweaken := by
+  simp [EType.tweaken, EType.cweaken, EType.crename_trename_comm]
+
 theorem TypedCont.tweaken
   (h : TypedCont Γ E t E') :
   TypedCont (Γ.tvar S) E.tweaken t.tweaken E'.tweaken := by
@@ -29,6 +33,14 @@ theorem TypedCont.tweaken
       rw [EType.tweaken_weaken] at ht1
       exact ht1 }
     { exact ih }
-  case conse => sorry
+  case conse ht _ ih =>
+    simp [Cont.tweaken]
+    simp [EType.tweaken_ex]
+    apply conse
+    { have ht1 := ht.tweaken_cext_ext (b := S)
+      rw [EType.tweaken_weaken] at ht1
+      rw [EType.tweaken_cweaken] at ht1
+      exact ht1 }
+    { exact ih }
 
 end Capless
